FlacTest.lean
@@ -1,1 +1,2 @@
+import FlacTest.Cli
 import FlacTest.Main
